Docs/LeanCompiler/STLC/Compile.lean
@@ -20,10 +20,10 @@ open LeanCompiler.STLC.CCify
   CcTerm (CpsTerm E)
 
 theorem compile_correct [TermParametricity] [PTermParametricity] (E : TermClosed .bool) :
-    CProgClosed.denote (compile E) (fun b => b) = TermClosed.denote E := by
+    CProgClosed.denote (compile E) (λ b => b) = TermClosed.denote E := by
   unfold compile
   simpa using Eq.trans
-    (CcTerm_correct (E := CpsTerm E) (k := fun b => b))
-    (CpsTerm_correct_bool (E := E) (k := fun b => b))
+    (CcTerm_correct (E := CpsTerm E) (k := λ b => b))
+    (CpsTerm_correct_bool (E := E) (k := λ b => b))
 
 end LeanCompiler.STLC.Compile
