Docs/LeanCompiler/STLC/Examples.lean
@@ -11,34 +11,34 @@ open LeanCompiler.STLC.CC
 local notation "BoolT" => Ty.bool
 
 def fals : TermClosed BoolT :=
-  fun _ => .fals
+  λ _ => .fals
 
 def tru : TermClosed BoolT :=
-  fun _ => .tru
+  λ _ => .tru
 
 def ident : TermClosed (BoolT ==> BoolT) :=
-  fun _ => .abs (fun x => .var x)
+  λ _ => .abs (λ x => .var x)
 
 def falsAgain : TermClosed BoolT :=
-  fun _ => .app (ident _) (fals _)
+  λ _ => .app (ident _) (fals _)
 
 def first : TermClosed (BoolT ==> BoolT ==> BoolT) :=
-  fun _ => .abs (fun x => .abs (fun _y => .var x))
+  λ _ => .abs (λ x => .abs (λ _y => .var x))
 
 def second : TermClosed (BoolT ==> BoolT ==> BoolT) :=
-  fun _ => .abs (fun _x => .abs (fun y => .var y))
+  λ _ => .abs (λ _x => .abs (λ y => .var y))
 
 def testFirst : TermClosed BoolT :=
-  fun _ => .app (.app (first _) (fals _)) (tru _)
+  λ _ => .app (.app (first _) (fals _)) (tru _)
 
 def testSecond : TermClosed BoolT :=
-  fun _ => .app (.app (second _) (fals _)) (tru _)
+  λ _ => .app (.app (second _) (fals _)) (tru _)
 
 def app : TermClosed ((BoolT ==> BoolT) ==> BoolT ==> BoolT) :=
-  fun _ => .abs (fun f => .abs (fun x => .app (.var f) (.var x)))
+  λ _ => .abs (λ f => .abs (λ x => .app (.var f) (.var x)))
 
 def falsAgain2 : TermClosed BoolT :=
-  fun _ => .app (.app (app _) (ident _)) (fals _)
+  λ _ => .app (.app (app _) (ident _)) (fals _)
 
 -- Source denotation checks.
 example : TermClosed.denote fals = false := rfl
@@ -79,10 +79,10 @@ def ccTestSecond := compile testSecond
 def ccApp := compile app
 def ccFalsAgain2 := compile falsAgain2
 
-example : CProgClosed.denote ccFals (fun b => b) = false := by
+example : CProgClosed.denote ccFals (λ b => b) = false := by
   simpa [ccFals, fals] using compile_correct fals
 
-example : CProgClosed.denote ccTestSecond (fun b => b) = true := by
+example : CProgClosed.denote ccTestSecond (λ b => b) = true := by
   simpa [ccTestSecond, testSecond, second, fals, tru, TermClosed.denote] using compile_correct testSecond
 
 end Parametric
